Lean4Lean/Verify/TypeChecker/IsDefEq.lean
@@ -323,8 +323,15 @@ theorem tryUnfoldProjApp.WF {c : VContext} {s : VState} (he : c.TrExprS e e') :
 def _root_.Lean4Lean.TypeChecker.ReductionStatus.WF
     (c : VContext) (e₁' e₂' : VExpr) (allowContinue := false) : ReductionStatus → Prop
   | .continue e₁ e₂ => allowContinue ∧ c.TrExpr e₁ e₁' ∧ c.TrExpr e₂ e₂'
-  | .unknown e₁ e₂ => c.TrExpr e₁ e₁' ∧ c.TrExpr e₂ e₂'
-  | .bool b => b → c.IsDefEqU e₁' e₂'
+  | .unknown e₁ e₂ | .false e₁ e₂ => c.TrExpr e₁ e₁' ∧ c.TrExpr e₂ e₂'
+  | .true => c.IsDefEqU e₁' e₂'
+
+theorem _root_.Lean4Lean.TypeChecker.ReductionStatus.WF.bool
+    (H1 : c.TrExpr e₁ e₁') (H2 : c.TrExpr e₂ e₂') (H : b = true → c.IsDefEqU e₁' e₂') :
+    ReductionStatus.WF c e₁' e₂' allowContinue (.bool e₁ e₂ b) :=
+  match b with
+  | .false => ⟨H1, H2⟩
+  | .true => H rfl
 
 def _root_.Lean4Lean.TypeChecker.ReductionStatus.WF.defeq
     (h1 : c.IsDefEqU e₁' e₁'') (h2 : c.IsDefEqU e₂' e₂'')
@@ -332,9 +339,9 @@ def _root_.Lean4Lean.TypeChecker.ReductionStatus.WF.defeq
   match r, H with
   | .continue .., ⟨a1, a2, a3⟩ =>
     ⟨a1, a2.defeq c.Ewf c.Δwf h1, a3.defeq c.Ewf c.Δwf h2⟩
-  | .unknown .., ⟨a2, a3⟩ =>
+  | .unknown .., ⟨a2, a3⟩ | .false .., ⟨a2, a3⟩ =>
     ⟨a2.defeq c.Ewf c.Δwf h1, a3.defeq c.Ewf c.Δwf h2⟩
-  | .bool _, h => fun hb => h1.symm.trans c.Ewf c.Δwf (h hb) |>.trans c.Ewf c.Δwf h2
+  | .true, h => h1.symm.trans c.Ewf c.Δwf h |>.trans c.Ewf c.Δwf h2
 
 theorem lazyDeltaReductionStep.WF {c : VContext} {s : VState}
     (he₁ : c.TrExprS e₁ e₁') (he₂ : c.TrExprS e₂ e₂') :
@@ -356,8 +363,8 @@ theorem lazyDeltaReductionStep.WF {c : VContext} {s : VState}
     let ⟨_, se₁, de₁⟩ := he₁; let ⟨_, se₂, de₂⟩ := he₂
     refine (quickIsDefEq.WF se₁ se₂).bind fun _ _ _ h => .pure ?_; split
     · exact ⟨rfl, he₁, he₂⟩
-    · intro; exact de₁.symm.trans c.Ewf c.Δwf (h rfl) |>.trans c.Ewf c.Δwf de₂
-    · nofun
+    · exact de₁.symm.trans c.Ewf c.Δwf (h rfl) |>.trans c.Ewf c.Δwf de₂
+    · exact ⟨he₁, he₂⟩
   split
   · exact .pure ⟨he₁.trExpr c.Ewf c.Δwf, he₂.trExpr c.Ewf c.Δwf⟩
   · refine (tryUnfoldProjApp.WF he₂).bind fun _ _ _ h => ?_; split
@@ -391,7 +398,7 @@ theorem lazyDeltaReductionStep.WF {c : VContext} {s : VState}
     (Level.isEquivList_wf h2 c2₁ c2₂)
   refine (isDefEqArgs.WF ⟨_, stk₁.tr, _, stk₂.tr, _, this⟩ he₁ he₂).bind fun _ _ _ h => ?_
   split <;> [skip; exact cacheFailure.WF.lift.bind fun _ _ _ _ => hF1]
-  exact .pure fun _ => h ‹_›
+  exact .pure <| h ‹_›
 
 theorem isNatZero_wf {c : VContext} (H : isNatZero e) (h : c.TrExprS e e') : e' = .natZero := by
   have h1 : c.TrExprS (.lit (.natVal 0)) e' := by
@@ -435,16 +442,19 @@ theorem lazyDeltaReduction.loop.WF {c : VContext} {s : VState}
   induction n generalizing s e₁ e₂ e₁' e₂' with | zero => exact .throw | succ n ih
   unfold loop; extract_lets F1
   refine (isDefEqOffset.WF he₁ he₂).bind fun _ _ _ h => ?_; split
-  · exact .pure fun hb => h (by simpa using hb)
+  · exact .pure <| .bool (he₁.trExpr c.Ewf c.Δwf) (he₂.trExpr c.Ewf c.Δwf) fun hb =>
+      h (by simpa using hb)
   suffices hF1 : ∀ {s}, (F1 ⟨⟩).WF c s fun r _ => r.WF c e₁' e₂' by
     refine .readThe ?_; split <;> [skip; exact hF1]
     refine (reduceNat.WF he₁).bind fun _ _ _ h => ?_; split
     · have ⟨_, a1, a2⟩ := (h _ rfl).2
-      refine (isDefEqCore.WF a1 he₂).bind fun _ _ _ h => .pure fun hb => ?_
+      refine (isDefEqCore.WF a1 he₂).bind fun _ _ _ h => ?_
+      refine .pure <| .bool ⟨_, a1, a2⟩ (he₂.trExpr c.Ewf c.Δwf) fun hb => ?_
       exact a2.symm.trans c.Ewf c.Δwf (h hb)
     refine (reduceNat.WF he₂).bind fun _ _ _ h => ?_; split
     · have ⟨_, a1, a2⟩ := (h _ rfl).2
-      refine (isDefEqCore.WF he₁ a1).bind fun _ _ _ h => .pure fun hb => ?_
+      refine (isDefEqCore.WF he₁ a1).bind fun _ _ _ h => ?_
+      refine .pure <| .bool (he₁.trExpr c.Ewf c.Δwf) ⟨_, a1, a2⟩ fun hb => ?_
       exact (h hb).trans c.Ewf c.Δwf a2
     exact hF1
   intro s; unfold F1; refine .getEnv ?_
@@ -453,11 +463,11 @@ theorem lazyDeltaReduction.loop.WF {c : VContext} {s : VState}
   refine (M.WF.liftExcept reduceNative.WF).lift.bind fun _ _ _ h => ?_
   split <;> [cases h _ rfl; skip]
   refine (lazyDeltaReductionStep.WF he₁ he₂).bind fun r _ _ h => ?_
-  obtain r|r|r := r
-  · let ⟨_, ⟨_, a1, a2⟩, ⟨_, b1, b2⟩⟩ := h
+  cases r with
+  | «continue» =>
+    let ⟨_, ⟨_, a1, a2⟩, ⟨_, b1, b2⟩⟩ := h
     exact (ih a1 b1).mono fun _ _ _ h => h.defeq a2 b2
-  · exact .pure h
-  · exact .pure h
+  | _ => exact .pure h
 
 theorem tryStringLitExpansionCore.WF {c : VContext} {s : VState}
     (he₁ : c.TrExprS e₁ e₁') (he₂ : c.TrExprS e₂ e₂') :
@@ -476,6 +486,44 @@ theorem tryStringLitExpansion.WF {c : VContext} {s : VState}
 theorem isDefEqUnitLike.WF {c : VContext} {s : VState}
     (he₁ : c.TrExprS e₁ e₁') (he₂ : c.TrExprS e₂ e₂') :
     RecM.WF c s (isDefEqUnitLike e₁ e₂) fun b _ => b = .true → c.IsDefEqU e₁' e₂' := sorry
+
+theorem lazyDeltaProjReduction.finish.WF {c : VContext} {s : VState}
+    (he₁ : c.TrExprS (.proj n₁ i e₁) e₁') (he₂ : c.TrExprS (.proj n₂ i e₂) e₂') :
+    (finish i e₁ e₂).WF c s fun r _ => r → c.IsDefEqU e₁' e₂' := by
+  unfold finish
+  refine (reduceProjCore.WF he₁).bind fun _ _ _ h1 => ?_; extract_lets F
+  have hF {s} : (F ⟨⟩).WF c s fun r _ => r → c.IsDefEqU e₁' e₂' := by
+    have .proj a1 a2 := he₁; have .proj b1 b2 := he₂
+    refine (isDefEqCore.WF a1 b1).mono fun _ _ _ h hb => ?_
+    exact a2.uniq c.Ewf (.refl c.Δwf.toCtx) b2 (h hb)
+  split <;> [have ⟨a1, _, a2, a3⟩ := h1 _ rfl; exact .pureBind hF]
+  refine (reduceProjCore.WF he₂).bind fun _ _ _ h2 => ?_
+  split <;> [have ⟨b1, _, b2, b3⟩ := h2 _ rfl; exact .pureBind hF]
+  exact (isDefEqCore.WF a2 b2).mono fun _ _ _ h hb =>
+    a3.symm.trans c.Ewf c.Δwf <| (h hb).trans c.Ewf c.Δwf b3
+
+theorem lazyDeltaProjReduction.loop.WF {c : VContext} {s : VState}
+    (he₁ : c.TrExprS (.proj n₁ i e₁) e₁') (he₂ : c.TrExprS (.proj n₂ i e₂) e₂') :
+    (loop i e₁ e₂ n).WF c s fun r _ => r → c.IsDefEqU e₁' e₂' := by
+  induction n generalizing s e₁ e₂ e₁' e₂' with | zero => exact .throw | succ n ih
+  unfold loop; have .proj a1 a2 := he₁; have .proj b1 b2 := he₂
+  refine (lazyDeltaReductionStep.WF a1 b1).bind fun _ _ _ h => ?_; split
+  · have ⟨_, ⟨_, c1, c2⟩, ⟨_, d1, d2⟩⟩ := h
+    have ⟨_, e1⟩ := a2.defeqDFC c.Ewf (.refl c.Δwf.toCtx) c2.symm
+    have ⟨_, e2⟩ := b2.defeqDFC c.Ewf (.refl c.Δwf.toCtx) d2.symm
+    refine (ih (.proj c1 e1) (.proj d1 e2)).mono fun _ _ _ h hb => ?_
+    have f1 := e1.uniq c.Ewf (.refl c.Δwf.toCtx) a2 c2
+    have f2 := e2.uniq c.Ewf (.refl c.Δwf.toCtx) b2 d2
+    exact f1.symm.trans c.Ewf c.Δwf <| (h hb).trans c.Ewf c.Δwf f2
+  · exact .pure fun _ => a2.uniq c.Ewf (.refl c.Δwf.toCtx) b2 h
+  all_goals
+    have ⟨⟨_, c1, c2⟩, ⟨_, d1, d2⟩⟩ := h
+    have ⟨_, e1⟩ := a2.defeqDFC c.Ewf (.refl c.Δwf.toCtx) c2.symm
+    have ⟨_, e2⟩ := b2.defeqDFC c.Ewf (.refl c.Δwf.toCtx) d2.symm
+    refine (finish.WF (.proj c1 e1) (.proj d1 e2)).mono fun _ _ _ h hb => ?_
+    have f1 := e1.uniq c.Ewf (.refl c.Δwf.toCtx) a2 c2
+    have f2 := e2.uniq c.Ewf (.refl c.Δwf.toCtx) b2 d2
+    exact f1.symm.trans c.Ewf c.Δwf <| (h hb).trans c.Ewf c.Δwf f2
 
 theorem isDefEqCore'.WF {c : VContext} {s : VState}
     (he₁ : c.TrExprS e₁ e₁') (he₂ : c.TrExprS e₂ e₂') :
@@ -514,7 +562,8 @@ theorem isDefEqCore'.WF {c : VContext} {s : VState}
   · exact .pure fun hb => h (by simpa using hb)
   refine (lazyDeltaReduction.loop.WF a1 b1).readThe.bind fun _ _ _ h => ?_; split
   · cases h.1
-  · exact .pure h
+  · exact .pure fun _ => h
+  · exact .pure nofun
   have ⟨⟨e₁', c1, c4⟩, ⟨e₂', d1, d4⟩⟩ := h
   refine .mono (Q := fun b _ => b = true → c.IsDefEqU e₁' e₂') ?_ fun _ _ _ h hb =>
     c4.symm.trans c.Ewf c.Δwf (h (by simpa using hb)) |>.trans c.Ewf c.Δwf d4
@@ -534,12 +583,9 @@ theorem isDefEqCore'.WF {c : VContext} {s : VState}
     · split <;> [rename_i h; exact this]
       simp at h; subst h
       exact .pure fun _ => c1.uniq c.Ewf (.refl c.Ewf c.Δwf) d1
-    · split <;> [rename_i h2; exact this]
-      have .proj c1 c2 := c1; have .proj d1 d2 := d1
-      refine (isDefEq.WF c1 d1).bind fun _ _ _ h => ?_
-      split <;> [skip; exact this]
-      simp at h2; subst h2; clear h
-      exact .pure fun _ => c2.uniq c.Ewf (.refl c.Δwf) d2 (h ‹_›)
+    · split <;> [rename_i h2; exact this]; simp at h2; subst h2
+      refine (lazyDeltaProjReduction.loop.WF c1 d1).bind fun _ _ _ h => ?_
+      split <;> [refine .pure fun _ => h ‹_›; exact this]
     · exact this
   intro; unfold F3
   refine (whnfCore.WF c1).bind fun _ _ _ ⟨_, e₁'', c5, c6⟩ => ?_
