Lean4Lean/Verify/TypeChecker/WHNF.lean
@@ -22,10 +22,6 @@ theorem whnfFVar.WF {c : VContext} {s : VState} (he : c.TrExprS (.fvar fv) e') :
   refine (TrExprS.fvar h1).uniq c.Ewf ?_ he
   exact .refl c.Ewf c.Δwf
 
-theorem reduceProj.WF {c : VContext} {s : VState} (he : c.TrExprS (.proj n i e) e') :
-    RecM.WF c s (reduceProj i e cheapProj) fun oe _ =>
-      ∀ e₁, oe = some e₁ → c.FVarsBelow (.proj n i e) e₁ ∧ c.TrExpr e₁ e' := sorry
-
 theorem whnfCore'.WF {c : VContext} {s : VState} (he : c.TrExprS e e') :
     RecM.WF c s (whnfCore' e cheapProj) fun e₁ _ =>
       c.FVarsBelow e e₁ ∧ c.TrExpr e₁ e' := by
